src/Example.Compile.Simple.fst
@@ -9,11 +9,30 @@ module XL = Pipit.Exec.LowStar
 
 module Tac = FStar.Tactics
 
+module Sugar = Pipit.SugarX4
+module C = Pipit.Context
+
+// noextract
+// let arg0_x: C.var bool = C.Var 100
+// noextract
+// let arg0: Pipit.Exp.Base.exp [] bool = Pipit.Exp.Base.XVar arg0_x
+
+// noextract
+// let extract_context (i: bool): XX.extract_context = {
+//   fv = (fun x -> if C.Var?.v x = C.Var?.v arg0_x
+//               then (C.cheat_variables_assume_global x arg0_x; Some i)
+//               else None);
+// }
+
+
 (* We will translate the "count_when" node with a variable as input.
    We do not want the expression's internal representation to show up in the
    C code, so we mark it as noextract. *)
 noextract
-let expr = (Simple.count_when (Pipit.Exp.XVar 0))
+let expr =
+  let open Sugar in
+  run1 (fun (i : s bool) ->
+    Simple.count_when i)
 
 (* Define the state type so it shows up as a type definition in the C code.
    The "postprocess_with" annotation ensures that the state_of_exp is inlined into the type and simplified to a regular type *)
@@ -22,7 +41,9 @@ let state = XX.state_of_exp expr
 
 (* Translate the expression to a transition system. *)
 noextract
-let system: Pipit.Exec.Base.exec (int * unit) state int = XX.exec_of_exp expr 1
+let system: Pipit.Exec.Base.exec (bool & unit) state int =
+  assert_norm (XX.extractable expr);
+  XX.exec_of_exp expr
 
 (* Define the reset function, which takes a pointer to the internal state and
    initialises it. *)
@@ -38,5 +59,6 @@ let reset = XL.mk_reset system
    variable of type (int * unit) rather than a pair constructors (inp, ()), some
    functions are not totally normalized.
    *)
-[@@(Tac.postprocess_with XL.tac_extract)]
-let step (inp: int) = XL.mk_step system (inp, ())
+[@@(Tac.postprocess_with (XL.tac_extract))]
+let step (inp: bool) = XL.mk_step system (inp, ())
+
