src/Pipit.Inhabited.fst
@@ -1,0 +1,13 @@
+module Pipit.Inhabited
+
+class inhabited (a: Type) = {
+  get_inhabited: a
+}
+
+instance inhabited_int: inhabited int = {
+  get_inhabited = 0;
+}
+
+instance inhabited_bool: inhabited bool = {
+  get_inhabited = false;
+}
